[WIP] Simplify semantics, tag SMTLib queries with their sort
Updated: Changes not propagated everywhere

vera/SMTLib.v
@@ -22,16 +22,17 @@ Import EqNotations.
 Import List.ListNotations.
 Local Open Scope list.
 
-(* Uninterpreted sorts *)
-Definition sort_sym := nat.
-
 Inductive sort : Set :=
 | Sort_Bool
-| Sort_Int
 (* SMTLIB says m > 0, but SMTCoq uses N in src/bva/BVList.v *)
 | Sort_BitVec (m : N)
-| Sort_Uninterpreted (_:sort_sym)
 .
+
+Definition interp_sort (s : sort) : Type :=
+match s with
+| Sort_Bool => bool
+| Sort_BitVec w => bitvector w
+end.
 
 (* Uninterpreted functions. Remarks:
    - predicate symbols are function symbols of codomain Bool
@@ -50,168 +51,51 @@ Variant BVBinOp : Set :=
   | BVXor
   | BVAdd
   | BVMul
-  | BVUDiv
-  | BVURem
+  (* | BVUDiv
+   * | BVURem *)
   | BVShl
   | BVShr
 .
 
-Inductive term : Type :=
-| Term_Const : const_sym -> term
-| Term_Int : Z -> term
-| Term_Geq : term -> term -> term
-| Term_Eq : term -> term -> term
-| Term_And : term -> term -> term
-| Term_Or : term -> term -> term
-| Term_Not : term -> term
-| Term_ITE : term -> term -> term -> term
-| Term_True : term
-| Term_False : term
-| Term_BVLit (w: N) : bitvector w -> term
-| Term_BVConcat : term -> term -> term
-| Term_BVExtract : nat -> nat -> term -> term
-| Term_BVUnaryOp : BVUnaryOp -> term -> term
-| Term_BVBinOp : BVBinOp -> term -> term -> term
-| Term_BVUlt : term -> term -> term
+Inductive term : sort -> Type :=
+(* Every constant reference is annotated. This corresponds to (as <var> <sort>) in SMTLIB. *)
+| Term_Const (s : sort) : const_sym -> term s
+| Term_Eq {s} : term s -> term s -> term Sort_Bool
+| Term_And : term Sort_Bool -> term Sort_Bool -> term Sort_Bool
+| Term_Or : term Sort_Bool -> term Sort_Bool -> term Sort_Bool
+| Term_Not : term Sort_Bool -> term Sort_Bool
+| Term_ITE {s : sort} : term Sort_Bool -> term s -> term s -> term s
+| Term_True : term Sort_Bool
+| Term_False : term Sort_Bool
+| Term_BVLit w : bitvector w -> term (Sort_BitVec w)
+| Term_BVConcat {w1 w2} : term (Sort_BitVec w1) -> term (Sort_BitVec w2) -> term (Sort_BitVec (w1 + w2))
+| Term_BVExtract {w} (hi lo : N) (wf : (lo <= hi)%N) : term (Sort_BitVec w) -> term (Sort_BitVec (1 + hi - lo))
+| Term_BVUnaryOp {w} : BVUnaryOp -> term (Sort_BitVec w) -> term (Sort_BitVec w)
+| Term_BVBinOp {w} : BVBinOp -> term (Sort_BitVec w) -> term (Sort_BitVec w) -> term (Sort_BitVec w)
+| Term_BVUlt {w} : term (Sort_BitVec w) -> term (Sort_BitVec w) -> term Sort_Bool
 .
 
 Definition dec_sort (s1 s2 : sort) : { s1 = s2 } + { s1 <> s2 }.
 Proof. repeat decide equality. Defined.
 
-(* To be able to interpret function symbol application, we introduce
-   an informative cast between sorts
-
-   See
-   https://www.lri.fr/~keller/Documents-recherche/Publications/thesis13.pdf
-   Sec.3.2.2 *)
-Section Cast.
-  Definition cast_result (A:Type) (n m:A) :=
-    option (forall (P:A -> Type), P n -> P m).
-  Definition idcast (A:Type) (n:A) : cast_result A n n :=
-    Some (fun P x => x).
-  Arguments idcast {A n}.
-
-  Fixpoint nat_cast (n m:nat) : cast_result nat n m :=
-    match n, m with
-    | O, O => idcast
-    | S n, S m =>
-        match nat_cast n m with
-        | Some k => Some (fun P => k (fun x => P (S x)))
-        | None => None
-        end
-    | _, _ => None
-    end.
-
-  Lemma nat_cast_refl:
-    forall n, nat_cast n n = idcast.
-  Proof. induction n as [ |n IHn]; simpl; try rewrite IHn; auto. Qed.
-
-  Fixpoint pos_cast (n m: positive) : cast_result positive n m :=
-    match n, m with
-    | xH, xH => idcast
-    | xO n, xO m =>
-        match pos_cast n m with
-        | Some k => Some (fun P => k (fun x => P (xO x)))
-        | None => None
-        end
-    | xI n, xI m =>
-        match pos_cast n m with
-        | Some k => Some (fun P => k (fun x => P (xI x)))
-        | None => None
-        end
-    | _, _ => None
-    end.
-
-  Lemma pos_cast_refl:
-    forall n, pos_cast n n = idcast.
-  Proof. induction n; simpl; try rewrite IHn; auto. Qed.
-
-  Definition N_cast (n m: N) : cast_result N n m :=
-    match n, m with
-    | N0, N0 => idcast
-    | Npos n, Npos m =>
-        match pos_cast n m with
-        | Some k => Some (fun P => k (fun x => P (Npos x)))
-        | None => None
-        end
-    | _, _ => None
-    end.
-
-  Lemma N_cast_refl:
-    forall n, N_cast n n = idcast.
-  Proof. induction n; simpl; try rewrite pos_cast_refl; try rewrite IHn; auto. Qed.
-
-  Definition cast (A B:sort) : cast_result sort A B :=
-    match A, B return cast_result sort A B with
-    | Sort_Bool, Sort_Bool => idcast
-    | Sort_Int, Sort_Int => idcast
-    | Sort_BitVec m1, Sort_BitVec m2 =>
-        match N_cast m1 m2 with
-        | Some k => Some (fun P => k (fun x => P (Sort_BitVec x)))
-        | None => None
-        end
-    | Sort_Uninterpreted n1, Sort_Uninterpreted n2 =>
-        match nat_cast n1 n2 with
-        | Some k => Some (fun P => k (fun x => P (Sort_Uninterpreted x)))
-        | None => None
-        end
-    | _, _ => None
-    end.
-
-  Lemma cast_refl:
-    forall s, cast s s = idcast.
-  Proof.
-    destruct s as [ | |m|n]; simpl; auto.
-    - now rewrite N_cast_refl.
-    - now rewrite nat_cast_refl.
-  Qed.
-End Cast.
+Definition valuation :=  forall (s : sort) (n : nat), interp_sort s.
 
 (* Interpretation *)
 Section Interpretation.
+  Definition value_eqb {s} : interp_sort s -> interp_sort s -> bool :=
+  match s as s' return interp_sort s' -> interp_sort s' -> bool with
+  | Sort_Bool => Bool.eqb
+  | Sort_BitVec w => @bv_eq w
+  end.
 
-  Variant value : Type :=
-    | Value_Bool (b : bool)
-    | Value_Int (i : Z)
-    | Value_BitVec (w : N) (bv : bitvector w)
-  .
-
-  Definition value_eqb (v1 v2 : value) : bool :=
-    match v1, v2 with
-    | Value_Bool b1, Value_Bool b2 => Bool.eqb b1 b2
-    | Value_Int z1, Value_Int z2 => Z.eqb z1 z2
-    | Value_BitVec w1 bv1, Value_BitVec w2 bv2 =>
-        match N.eq_dec w1 w2 with
-        | left eq => bv_eq bv1 (rew <- eq in bv2)
-        | right _ => false
-        end
-    | _, _ => false
-    end.
-
-  Lemma value_eqb_eq v1 v2 : value_eqb v1 v2 = true <-> v1 = v2.
+  Lemma value_eqb_eq s v1 v2 : @value_eqb s v1 v2 = true <-> v1 = v2.
   Proof.
-    split; intros H.
-    - destruct v1, v2; simpl in *; try discriminate.
-      + rewrite Bool.eqb_true_iff in H. subst.
-        reflexivity.
-      + rewrite Z.eqb_eq in H. subst.
-        reflexivity.
-      + destruct (N.eq_dec w w0); try discriminate.
-        subst.
-        replace (rew <- [bitvector] eq_refl in bv1) with bv1 in H by reflexivity.
-        apply bv_eq_reflect in H. subst.
-        reflexivity.
-    - subst.
-      destruct v2; simpl.
-      + rewrite Bool.eqb_true_iff. reflexivity.
-      + rewrite Z.eqb_eq. reflexivity.
-      + destruct (N.eq_dec w w); try contradiction.
-        dependent destruction e.
-        replace (rew <- [bitvector] eq_refl in bv0) with bv0 by reflexivity.
-        apply bv_eq_refl.
+    destruct s; simpl in *.
+    - apply Bool.eqb_true_iff.
+    - apply bv_eq_reflect.
   Qed.
 
-  Lemma value_eqb_refl v : value_eqb v v = true.
+  Lemma value_eqb_refl s v : @value_eqb s v v = true.
   Proof. apply value_eqb_eq. reflexivity. Qed.
 
   (* TODO: This is probably wrong. *)
@@ -250,121 +134,54 @@ Section Interpretation.
   Qed.
 
   (* Interpretation of terms *)
-  Variable interp_const_sym : nat -> option value.
+  Variable ρ : valuation.
 
-  Fixpoint interp_term (t:term) : option value :=
+  Fixpoint interp_term {s} (t:term s) : (interp_sort s) :=
     match t with
     (* TODO: uninterpreted functions *)
-    | Term_Const n => interp_const_sym n
-    | Term_Int z => Some (Value_Int z)
-    | Term_Geq t1 t2 =>
-        match interp_term t1, interp_term t2 with
-        | Some (Value_Int z1), Some (Value_Int z2) =>
-            Some (Value_Bool (z1 >=? z2)%Z)
-        | _, _ => None
-        end
+    | Term_Const s n => ρ s n
     | Term_Eq t1 t2 =>
-        match interp_term t1, interp_term t2 with
-        | Some v1, Some v2 =>
-            Some (Value_Bool (value_eqb v1 v2))
-        | _, _ => None
-        end
-    | Term_And t1 t2 =>
-        match interp_term t1, interp_term t2 with
-        | Some (Value_Bool b1), Some (Value_Bool b2) =>
-            Some (Value_Bool (b1 && b2)%bool)
-        | _, _ => None
-        end
+	value_eqb (interp_term t1) (interp_term t2)
+    | Term_And t1 t2 => ((interp_term t1) && (interp_term t2))%bool
     | Term_Or t1 t2 =>
-        match interp_term t1, interp_term t2 with
-        | Some (Value_Bool b1), Some (Value_Bool b2) =>
-            Some (Value_Bool (b1 || b2)%bool)
-        | _, _ => None
-        end
-    | Term_Not t =>
-        match interp_term t with
-        | Some (Value_Bool b) => Some (Value_Bool (negb b))
-        | _ => None
-        end
+      ((interp_term t1) || (interp_term t2))%bool
+    | Term_Not t => negb (interp_term t)
     | Term_ITE t1 t2 t3 =>
-        match interp_term t1, interp_term t2, interp_term t3 with
-        | Some (Value_Bool b1), Some v2, Some v3 =>
-            if b1 then Some v2 else Some v3
-        | _, _, _ => None
-        end
-    | Term_True => Some (Value_Bool true)
-    | Term_False => Some (Value_Bool false)
-    | Term_BVLit w bv =>
-        Some (Value_BitVec w bv)
+      if interp_term t1 then interp_term t2 else interp_term t3
+    | Term_True => true
+    | Term_False => false
+    | Term_BVLit w bv => bv
     | Term_BVConcat t1 t2 =>
-        match interp_term t1, interp_term t2 with
-        | Some (Value_BitVec m1 bv1), Some (Value_BitVec m2 bv2) =>
-            Some (Value_BitVec (m1 + m2) (bv_concat bv1 bv2))
-        | _, _ => None
-        end
-    | Term_BVExtract hi lo t =>
-        match interp_term t with
-        | Some (Value_BitVec m bv) =>
-            if (lo <=? hi)
-            then Some (Value_BitVec (N_of_nat (hi - lo + 1)) (bv_extr (N_of_nat lo) _ bv))
-            else None
-        | _ => None
-        end
+      bv_concat (interp_term t1) (interp_term t2)
+    | Term_BVExtract hi lo _ t =>
+      bv_extr lo _ (interp_term t)
     | Term_BVUnaryOp op t =>
-        match interp_term t with
-        | Some (Value_BitVec m bv) =>
-            match op with
-            | BVNot => Some (Value_BitVec m (bv_not bv))
-            | BVNeg => Some (Value_BitVec m (bv_neg bv))
-            end
-        | _ => None
-        end
+      match op with
+      | BVNot => bv_not (interp_term t)
+      | BVNeg => bv_neg (interp_term t)
+      end
     | Term_BVBinOp binop t1 t2 =>
-        match interp_term t1, interp_term t2 with
-        | Some (Value_BitVec m1 bv1),
-          Some (Value_BitVec m2 bv2_2) =>
-            match N.eq_dec m2 m1 with
-            | left e =>
-                let bv2 : bitvector m1 := eq_rect m2 bitvector bv2_2 m1 e in
-                match binop with
-                | BVAnd => Some (Value_BitVec m1 (bv_and bv1 bv2))
-                | BVOr =>  Some (Value_BitVec m1 (bv_or bv1 bv2))
-		(* TODO: Follow standard more precisely. This should be an abbreviation:
-		     (bvxor s t) abbreviates (bvor (bvand s (bvnot t)) (bvand (bvnot s) t))
-		*)
-                | BVXor =>  Some (Value_BitVec m1 (bv_xor bv1 bv2))
-                | BVAdd => Some (Value_BitVec m1 (bv_add bv1 bv2))
-                | BVMul => Some (Value_BitVec m1 (bv_mult bv1 bv2))
-                | BVUDiv =>
-                    (* Divide does not exist in SMTCoq bitvectors *)
-                    (* Some (existT _ (Sort_BitVec m1) (bv_udiv bv1 bv2)) *)
-                    None
-                | BVURem =>
-                    (* Divide does not exist in SMTCoq bitvectors *)
-                    (* Some (existT _ (Sort_BitVec m1) (bv_rem bv1 bv2)) *)
-                    None
-                | BVShl => Some (Value_BitVec m1 (bv_shl bv1 bv2))
-                | BVShr => Some (Value_BitVec m1 (bv_shr bv1 bv2))
-                end
-            | right _ => None
-            end
-        | _, _ => None
-        end
+      match binop with
+      | BVAnd => bv_and (interp_term t1) (interp_term t2)
+      | BVOr => bv_or (interp_term t1) (interp_term t2)
+      (* TODO: Follow standard more precisely. This should be an abbreviation:
+      (bvxor s t) abbreviates (bvor (bvand s (bvnot t)) (bvand (bvnot s) t))
+      *)
+      | BVXor => bv_xor (interp_term t1) (interp_term t2)
+      | BVAdd => bv_add (interp_term t1) (interp_term t2)
+      | BVMul => bv_mult (interp_term t1) (interp_term t2)
+      (* Divide does not exist in SMTCoq bitvectors *)
+      (* (existT _ (Sort_BitVec m1) (bv_udiv (interp_term t1) (interp_term t2))) *)
+      (* (existT _ (Sort_BitVec m1) (bv_rem (interp_term t1) (interp_term t2))) *)
+      (* | BVUDiv => None
+       * | BVURem => None *)
+      | BVShl => bv_shl (interp_term t1) (interp_term t2)
+      | BVShr => bv_shr (interp_term t1) (interp_term t2)
+      end
     | Term_BVUlt t1 t2 =>
-        match interp_term t1, interp_term t2 with
-        | Some (Value_BitVec m1 bv1),
-          Some (Value_BitVec m2 bv2) =>
-            if (m1 =? m2)%N
-            then Some (Value_Bool (bv2nat bv1 <=? bv2nat bv2))
-            else None
-        | _, _ => None
-        end
+      (bv2nat (interp_term t1) <=? bv2nat (interp_term t2))
     end.
 
-  Definition interp_formula (t:term) : bool :=
-    match interp_term t with
-    | Some (Value_Bool b) => b
-    | _ => true
-    end.
+  Definition interp_formula (t:term Sort_Bool) : bool := interp_term t.
 
 End Interpretation.
