vera/VerilogSMT.v
@@ -117,68 +117,45 @@ Module SMT.
       }.
 
   Definition max_declaration (q : SMTQueries.query) : nat :=
-    List.list_max (List.map fst (SMTQueries.declarations q)).
-
-  Lemma max_declaration_declarations q name s :
-    In (name, s) (SMTQueries.declarations q) ->
-    name <= max_declaration q.
-  Proof.
-    unfold max_declaration, SMTQueries.domain.
-    destruct q. simpl in *. rewrite List.Forall_forall in *.
-    intros Hin_domain. clear wf0. clear assertions.
-    revert name s Hin_domain.
-    induction declarations; [crush|].
-    intros.
-    inv Hin_domain; simpl in *; [lia|].
-    insterU IHdeclarations.
-    lia.
-  Qed.
+    List.list_max (SMTQueries.domain q).
 
   Lemma max_declaration_domain q name :
     In name (SMTQueries.domain q) ->
     name <= max_declaration q.
   Proof.
-    intros Hin_domain.
-    pose proof (SMTQueries.wf q) as wf.
-    rewrite List.Forall_forall in wf.
-    edestruct wf as [s Hin_decls]; [eassumption|].
-    eapply max_declaration_declarations.
-    eassumption.
+    unfold max_declaration, SMTQueries.domain.
+    revert name. rewrite <- Forall_forall.
+    apply list_max_le.
+    trivial.
   Qed.
-
-  Program Definition valuation_of_execution (tag : TaggedVariable.Tag) (m : VerilogSMTBijection.t) (e : execution) : SMTQueries.valuation :=
-    fun n =>
-      match bij_inverse m n with
-      | None => None
-      | Some (t, vname) =>
-          if dec (t = tag)
-          then
-            match e vname with
-            | None => None
-            | Some x =>
-                match XBV.to_bv x with
-                (* TODO: Fix handling of Xs *)
-                | None => None
-                | Some val => Some (SMTLib.Value_BitVec _ val)
-                end
-            end
-          else None
-      end.
 
   Import EqNotations.
 
-  Definition execution_of_valuation (tag : TaggedVariable.Tag) (m : VerilogSMTBijection.t) (v : SMTQueries.valuation) : execution :=
+  Definition valuation_of_execution (tag : TaggedVariable.Tag) (m : VerilogSMTBijection.t) (e : execution) : SMTLib.valuation :=
+    fun s n =>
+      match s as s' return SMTLib.interp_sort s' with
+      | SMTLib.Sort_Bool => false
+      | SMTLib.Sort_BitVec w => 
+        match bij_inverse m n with
+        | None => BV.zeros w
+        | Some (t, vname) =>
+	  match dec (t = tag), dec (Verilog.varType vname = w), e vname with
+	  | left _, left E, Some x =>
+            match XBV.to_bv x with
+            (* TODO: Fix handling of Xs *)
+            | None => BV.zeros w
+            | Some val => rew E in val
+	    end
+	  | _, _, _ => BV.zeros w
+          end
+        end
+      end.
+
+  Definition execution_of_valuation (tag : TaggedVariable.Tag) (m : VerilogSMTBijection.t) (v : SMTLib.valuation) : execution :=
     fun var =>
       match m (tag, var) with
       | Some smtName =>
-          match v smtName with
-          | Some (SMTLib.Value_BitVec w bv) =>
-              match dec (w = Verilog.varType var) with
-              | left e => Some (rew e in (XBV.from_bv bv))
-              | _ => None
-              end
-          | _ => None
-          end
+        Some (XBV.from_bv (v (SMTLib.Sort_BitVec (Verilog.varType var)) smtName))
       | None => None
       end
   .
@@ -196,160 +173,38 @@ Module SMT.
     discriminate.
   Qed.
 
-  Lemma execution_of_valuation_some tag (m : VerilogSMTBijection.t) ρ smtName var bv :
+  Lemma execution_of_valuation_some tag (m : VerilogSMTBijection.t) ρ smtName var :
     m (tag, var) = Some smtName ->
-    ρ smtName = Some (SMTLib.Value_BitVec (Verilog.varType var) bv) ->
-    execution_of_valuation tag m ρ var = Some (XBV.from_bv bv).
+    execution_of_valuation tag m ρ var = Some (XBV.from_bv (ρ (SMTLib.Sort_BitVec (Verilog.varType var)) smtName)).
   Proof.
     unfold execution_of_valuation.
-    intros H1 H2.
-    rewrite H1; rewrite H2.
-    autodestruct; [|contradiction].
-    now rewrite <- eq_rect_eq.
+    intros H1. rewrite H1.
+    reflexivity.
   Qed.
 
-  Definition valuation_of_executions (m : VerilogSMTBijection.t) (e1 e2 : execution) : SMTQueries.valuation :=
-    fun n =>
-      match bij_inverse m n with
-      | None => None
-      | Some (tag, var) =>
-          let e :=
-            match tag with
-            | TaggedVariable.VerilogLeft => e1
-            | TaggedVariable.VerilogRight => e2
-            end
-          in
-          match e var with
-          | None => None
-          | Some xbv =>
-              match XBV.to_bv xbv with
-              (* TODO: Fix handling of Xs *)
-              | None => None
-              | Some val => Some (SMTLib.Value_BitVec _ val)
+  Definition valuation_of_executions (m : VerilogSMTBijection.t) (e1 e2 : execution) : SMTLib.valuation :=
+    fun s n =>
+      match s as s' return SMTLib.interp_sort s' with
+      | SMTLib.Sort_Bool => false 
+      | SMTLib.Sort_BitVec w => 
+        match bij_inverse m n with
+        | None => BV.zeros w
+        | Some (tag, var) =>
+            let e :=
+              match tag with
+              | TaggedVariable.VerilogLeft => e1
+              | TaggedVariable.VerilogRight => e2
               end
-          end
+            in
+            match dec (Verilog.varType var = w), e var with
+            | left E, Some xbv =>
+                match XBV.to_bv xbv with
+                (* TODO: Fix handling of Xs *)
+                | None => BV.zeros w
+                | Some val => rew E in val
+                end
+            | _, _ => BV.zeros w
+            end
+        end
       end.
-
-  Lemma execution_left_of_valuation_of_executions m v e1 e2 :
-    (* TODO: Remove assumption *)
-    (forall n xbv, e1 n = Some xbv -> ~ XBV.has_x xbv) ->
-    (forall n xbv, e2 n = Some xbv -> ~ XBV.has_x xbv) ->
-    match_map_vars TaggedVariable.VerilogLeft m (Verilog.modVariables v) ->
-    complete_execution v e1 ->
-    execution_of_valuation TaggedVariable.VerilogLeft m (valuation_of_executions m e1 e2) = e1.
-  Proof.
-    intros * Hno_exes1 Hno_exes2 Hmatch Hcomplete.
-    unfold valuation_of_executions.
-    unfold execution_of_valuation.
-    apply functional_extensionality_dep.
-    intros [varName varType].
-    autodestruct_eqn E;
-      simpl in *; try subst; repeat apply_somewhere inj_pair2; try subst.
-    - destruct v1 as [n1 t1]. simpl in *.
-      replace n1 with varName in * by (apply bij_wf in E; crush).
-      simpl in *.
-      replace (e1 {| Verilog.varName := varName; Verilog.varType := t1 |}). repeat f_equal.
-      apply XBV.bv_xbv_inverse. assumption.
-    - destruct v1 as [n1 t1]. simpl in *.
-      replace n1 with varName in * by (apply bij_wf in E; crush).
-      rewrite bij_wf in *. congruence.
-    - rewrite bij_wf in *. congruence.
-    - rewrite bij_wf in *. congruence.
-    - destruct v0 as [n1 t1]. simpl in *. replace n1 with varName in * by (apply bij_wf in E; crush).
-      apply_somewhere (Hno_exes1 {| Verilog.varName := varName; Verilog.varType := t1 |}).
-      now rewrite <- XBV.has_x_to_bv in *.
-    - destruct v0 as [n1 t1]. simpl in *. replace n1 with varName in * by (apply bij_wf in E; crush).
-      apply_somewhere (Hno_exes2 {| Verilog.varName := varName; Verilog.varType := t1 |}).
-      now rewrite <- XBV.has_x_to_bv in *.
-    - destruct v0 as [n1 t1]. simpl in *.
-      replace n1 with varName in * by (apply bij_wf in E; crush).
-      replace t1 with varType in * by (apply bij_wf in E; crush).
-      crush.
-    - destruct v0 as [n1 t1]. simpl in *.
-      replace n1 with varName in * by (apply bij_wf in E; crush).
-      replace t1 with varType in * by (apply bij_wf in E; crush).
-      rewrite bij_wf in *; congruence.
-    - rewrite bij_wf in *; congruence.
-    - admit.
-  Admitted.
-
-  Lemma execution_right_of_valuation_of_executions m v e1 e2 :
-    (* TODO: Remove assumption *)
-    (forall n xbv, e1 n = Some xbv -> ~ XBV.has_x xbv) ->
-    (forall n xbv, e2 n = Some xbv -> ~ XBV.has_x xbv) ->
-    match_map_vars TaggedVariable.VerilogRight m (Verilog.modVariables v) ->
-    complete_execution v e2 ->
-    execution_of_valuation TaggedVariable.VerilogRight m (valuation_of_executions m e1 e2) = e2.
-  Proof. Admitted.
-
-  Lemma valuation_of_executions_some_left var nameSMT xbv bv (m : VerilogSMTBijection.t) e1 e2 :
-    e1 var = Some xbv ->
-    XBV.to_bv xbv = Some bv ->
-    m (TaggedVariable.VerilogLeft, var) = Some nameSMT ->
-    (valuation_of_executions m e1 e2) nameSMT =
-      Some (SMTLib.Value_BitVec (Verilog.varType var) bv).
-  Proof.
-    intros Hexec Hexes Hname.
-    unfold valuation_of_executions; simpl.
-
-    pose proof (bij_wf m) as Hinverse.
-    specialize (Hinverse (TaggedVariable.VerilogLeft, var) nameSMT).
-    apply Hinverse in Hname. clear Hinverse.
-    rewrite Hname.
-
-    rewrite Hexec.
-    rewrite Hexes.
-    reflexivity.
-  Qed.
-
-  Lemma valuation_of_executions_some_right var nameSMT xbv bv (m : VerilogSMTBijection.t) e1 e2 :
-    e2 var = Some xbv ->
-    XBV.to_bv xbv = Some bv ->
-    m (TaggedVariable.VerilogRight, var) = Some nameSMT ->
-    (valuation_of_executions m e1 e2) nameSMT =
-      Some (SMTLib.Value_BitVec (Verilog.varType var) bv).
-  Proof.
-    intros Hexec Hexes Hname.
-    unfold valuation_of_executions; simpl.
-
-    pose proof (bij_wf m) as Hinverse.
-    specialize (Hinverse (TaggedVariable.VerilogRight, var) nameSMT).
-    apply Hinverse in Hname. clear Hinverse.
-    rewrite Hname.
-
-    rewrite Hexec.
-    rewrite Hexes.
-    reflexivity.
-  Qed.
-
-  Section inverse.
-    Variable m : VerilogSMTBijection.t.
-    Variable v : Verilog.vmodule.
-    Variable e : execution.
-    Variable tag : TaggedVariable.Tag.
-    Context (Hcomplete : complete_execution v e).
-    Context (Hmatch : match_map_vars tag m (Verilog.modVariables v)).
-
-    Lemma valuation_of_execution_some var nameSMT xbv bv :
-      e var = Some (xbv) ->
-      XBV.to_bv xbv = Some bv ->
-      m (tag, var) = Some nameSMT ->
-      (valuation_of_execution tag m e) nameSMT =
-        Some (SMTLib.Value_BitVec (Verilog.varType var) bv).
-    Proof.
-      intros Hexec Hexes Hname.
-      unfold valuation_of_execution; simpl.
-
-      pose proof (bij_wf m) as Hinverse.
-      specialize (Hinverse (tag, var) nameSMT).
-      apply Hinverse in Hname.
-      rewrite Hname.
-
-      destruct (dec (tag = tag)); [|contradiction].
-
-      rewrite Hexec.
-      rewrite Hexes.
-      reflexivity.
-    Qed.
-  End inverse.
 End SMT.
