vera/VerilogToSMT/VerilogToSMT.v
@@ -23,6 +23,7 @@ From ExtLib Require Import Structures.Traversable.
 From ExtLib Require Import Programming.Show.
 
 From vera Require SMTLib.
+Import SMTLib (Sort_BitVec, Sort_Bool).
 
 From vera Require Import Verilog.
 From vera Require Import Common.
@@ -40,6 +41,7 @@ Import ListNotations.
 Import CommonNotations.
 Import MonadLetNotation.
 Import FunctorNotation.
+Import EqNotations.
 Local Open Scope monad_scope.
 
 Local Definition smtname := nat.
@@ -47,14 +49,17 @@ Local Definition width := N.
 
 Definition transf := sum string.
 
-Equations cast_from_to (from to: N) (t : SMTLib.term) : SMTLib.term :=
-  cast_from_to from to t with N.compare to from => {
-    | Lt => SMTLib.Term_BVExtract (N.to_nat to - 1) 0 t
-    (* smtlib concat is backwards *)
-    | Gt => SMTLib.Term_BVConcat (SMTLib.Term_BVLit _ (BV.zeros (to - from))) t
-    | Eq => t
+Local Obligation Tactic := intros.
+Equations cast_from_to (from to: N) (t : SMTLib.term (Sort_BitVec from)) : SMTLib.term (Sort_BitVec to) :=
+  cast_from_to from 0 t => SMTLib.Term_BVLit _ (BV.of_bits []);
+  cast_from_to from to t with dec (from < to)%N => {
+    | left lt => rew _ in SMTLib.Term_BVConcat (SMTLib.Term_BVLit _ (BV.zeros (to - from))) t
+    | right ge => rew _ in SMTLib.Term_BVExtract (to - 1) 0 _ t
     }
 .
+Next Obligation. f_equal. lia. Qed.
+Next Obligation. f_equal. lia. Qed.
+Next Obligation. f_equal. lia. Qed.
 
 Definition static_value {w} (expr : Verilog.expression w) : option (BV.bitvector w) :=
   match expr with
@@ -75,85 +80,78 @@ Section expr_to_smt.
   Variable inputs : list Verilog.variable.
   Variable outputs : list Verilog.variable.
 
-  Equations var_to_smt (var : Verilog.variable): transf SMTLib.term :=
+  Equations var_to_smt (var : Verilog.variable): transf (SMTLib.term (Sort_BitVec (Verilog.varType var))) :=
     var_to_smt var with name_bijection (tag, var) := {
       | None => raise ("Name not declared: " ++ (Verilog.varName var))%string
-      | Some n_smt => ret (SMTLib.Term_Const n_smt)
+      | Some n_smt => ret (SMTLib.Term_Const _ n_smt)
       }.
 
   Definition smt_select_bit vec_width vec_smt idx_width idx_smt :=
-    SMTLib.Term_BVExtract 0 0
+    SMTLib.Term_BVExtract 0 0 ltac:(lia)
       (SMTLib.Term_BVBinOp SMTLib.BVShr
          (cast_from_to vec_width (N.max vec_width idx_width) vec_smt)
          (cast_from_to idx_width (N.max vec_width idx_width) idx_smt)).
 
-  Equations arithmeticop_to_smt : Verilog.arithmeticop -> SMTLib.term -> SMTLib.term -> transf SMTLib.term :=
+  Equations arithmeticop_to_smt {w} :
+      Verilog.arithmeticop ->
+      SMTLib.term (Sort_BitVec w) ->
+      SMTLib.term (Sort_BitVec w) ->
+      (SMTLib.term (Sort_BitVec w)) :=
     arithmeticop_to_smt Verilog.ArithmeticPlus lhs rhs :=
-      ret (SMTLib.Term_BVBinOp SMTLib.BVAdd lhs rhs);
+      SMTLib.Term_BVBinOp SMTLib.BVAdd lhs rhs;
     arithmeticop_to_smt Verilog.ArithmeticMinus lhs rhs :=
-      ret (SMTLib.Term_BVBinOp SMTLib.BVAdd lhs (SMTLib.Term_BVUnaryOp SMTLib.BVNeg rhs));
+      SMTLib.Term_BVBinOp SMTLib.BVAdd lhs (SMTLib.Term_BVUnaryOp SMTLib.BVNeg rhs);
     arithmeticop_to_smt Verilog.ArithmeticStar lhs rhs :=
-      ret (SMTLib.Term_BVBinOp SMTLib.BVMul lhs rhs);
+      SMTLib.Term_BVBinOp SMTLib.BVMul lhs rhs;
     .
 
-  Equations shiftop_to_smt : Verilog.shiftop -> SMTLib.term -> SMTLib.term -> transf SMTLib.term :=
+  Equations shiftop_to_smt {w} : Verilog.shiftop -> SMTLib.term (Sort_BitVec w) -> SMTLib.term (Sort_BitVec w) -> (SMTLib.term (Sort_BitVec w)) :=
     shiftop_to_smt Verilog.BinaryShiftLeft lhs rhs :=
-      ret (SMTLib.Term_BVBinOp SMTLib.BVShl lhs rhs);
+      (SMTLib.Term_BVBinOp SMTLib.BVShl lhs rhs);
     shiftop_to_smt Verilog.BinaryShiftLeftArithmetic lhs rhs :=
-      ret (SMTLib.Term_BVBinOp SMTLib.BVShl lhs rhs);
+      (SMTLib.Term_BVBinOp SMTLib.BVShl lhs rhs);
     shiftop_to_smt Verilog.BinaryShiftRight lhs rhs :=
-      ret (SMTLib.Term_BVBinOp SMTLib.BVShr lhs rhs);
+      (SMTLib.Term_BVBinOp SMTLib.BVShr lhs rhs);
   .
 
-  Equations bitwiseop_to_smt : Verilog.bitwiseop -> SMTLib.term -> SMTLib.term -> transf SMTLib.term :=
+  Equations bitwiseop_to_smt {w} : Verilog.bitwiseop -> SMTLib.term (Sort_BitVec w) -> SMTLib.term (Sort_BitVec w) -> SMTLib.term (Sort_BitVec w) :=
     bitwiseop_to_smt Verilog.BinaryBitwiseOr lhs rhs :=
-      ret (SMTLib.Term_BVBinOp SMTLib.BVOr lhs rhs);
+      SMTLib.Term_BVBinOp SMTLib.BVOr lhs rhs;
     bitwiseop_to_smt Verilog.BinaryBitwiseXor lhs rhs :=
-      ret (SMTLib.Term_BVBinOp SMTLib.BVXor lhs rhs);
+      SMTLib.Term_BVBinOp SMTLib.BVXor lhs rhs;
     bitwiseop_to_smt Verilog.BinaryBitwiseAnd lhs rhs :=
-      ret (SMTLib.Term_BVBinOp SMTLib.BVAnd lhs rhs)
+      SMTLib.Term_BVBinOp SMTLib.BVAnd lhs rhs
   .
 
-  Equations unaryop_to_smt : Verilog.unaryop -> SMTLib.term -> transf SMTLib.term :=
+  Equations unaryop_to_smt {w} : Verilog.unaryop -> SMTLib.term (Sort_BitVec w) -> (SMTLib.term (Sort_BitVec w)) :=
     unaryop_to_smt Verilog.UnaryPlus operand :=
-      ret operand ;
+      operand ;
     (* unaryop_to_smt Verilog.UnaryMinus operand := *)
     (*   ret (SMTLib.Term_BVUnaryOp SMTLib.BVNeg operand); *)
     unaryop_to_smt Verilog.UnaryNot operand :=
-      ret (SMTLib.Term_BVUnaryOp SMTLib.BVNot operand)
+      (SMTLib.Term_BVUnaryOp SMTLib.BVNot operand)
   .
 
-  Definition conditional_to_smt
-    (cond_type : Verilog.vtype) (cond ifT ifF : SMTLib.term) : SMTLib.term :=
+  Definition conditional_to_smt {w_val}
+    (cond_type : Verilog.vtype) (cond : SMTLib.term (Sort_BitVec cond_type)) (ifT ifF : SMTLib.term (Sort_BitVec w_val))
+    : SMTLib.term (Sort_BitVec w_val) :=
     SMTLib.Term_ITE
       (SMTLib.Term_Not (SMTLib.Term_Eq cond (SMTLib.Term_BVLit _ (BV.zeros cond_type))))
       ifT ifF
   .
 
-  Definition sign_extend (from to : N) (term : SMTLib.term) :=
-    let added_width := (to - from)%N in
-    let msb := N.to_nat (from - 1)%N in
-    if (N.eqb added_width 0%N)
-    then term
-    else
-    SMTLib.Term_ITE
-      (SMTLib.Term_Eq (SMTLib.Term_BVExtract msb msb term) (SMTLib.Term_BVLit 1 (BV.zeros 1)))
-      (SMTLib.Term_BVConcat term (SMTLib.Term_BVLit _ (BV.zeros added_width)))
-      (SMTLib.Term_BVConcat term (SMTLib.Term_BVLit _ (BV.ones added_width)))
-      .
-
-  Equations expr_to_smt {w} : Verilog.expression w -> transf SMTLib.term :=
+  Equations expr_to_smt {w} : Verilog.expression w -> transf (SMTLib.term (Sort_BitVec w)) :=
     expr_to_smt (Verilog.UnaryOp op operand) :=
       let* operand_smt := expr_to_smt operand in
-      unaryop_to_smt op operand_smt ;
+      ret (unaryop_to_smt op operand_smt) ;
     expr_to_smt (Verilog.ArithmeticOp op lhs rhs) :=
       let* lhs_smt := expr_to_smt lhs in
       let* rhs_smt := expr_to_smt rhs in
-      arithmeticop_to_smt op lhs_smt rhs_smt;
+      ret (arithmeticop_to_smt op lhs_smt rhs_smt);
     expr_to_smt (Verilog.BitwiseOp op lhs rhs) :=
       let* lhs_smt := expr_to_smt lhs in
       let* rhs_smt := expr_to_smt rhs in
-      bitwiseop_to_smt op lhs_smt rhs_smt;
+      ret (bitwiseop_to_smt op lhs_smt rhs_smt);
     expr_to_smt (Verilog.ShiftOp op lhs rhs _ _) :=
       let* lhs_smt_short := expr_to_smt lhs in
       let* rhs_smt_short := expr_to_smt rhs in
@@ -165,7 +163,7 @@ Section expr_to_smt.
       let op_width := N.max lhs_width rhs_width in
       let lhs_smt := cast_from_to lhs_width op_width lhs_smt_short in
       let rhs_smt := cast_from_to rhs_width op_width rhs_smt_short in
-      let* long_result := shiftop_to_smt op lhs_smt rhs_smt in
+      let long_result := shiftop_to_smt op lhs_smt rhs_smt in
       ret (cast_from_to op_width lhs_width long_result);
     expr_to_smt (Verilog.Concatenation e1 e2) :=
       let* e1_smt := expr_to_smt e1 in
@@ -179,9 +177,9 @@ Section expr_to_smt.
       let* ifT_smt := expr_to_smt ifT in
       let* ifF_smt := expr_to_smt ifF in
       ret (conditional_to_smt cond_type cond_smt ifT_smt ifF_smt);
-    expr_to_smt (Verilog.RangeSelect vec hi lo _ _) :=
+    expr_to_smt (Verilog.RangeSelect vec hi lo _ wf) :=
       let* vec_smt := expr_to_smt vec in
-      ret (SMTLib.Term_BVExtract (N.to_nat hi) (N.to_nat lo) vec_smt);
+      ret (SMTLib.Term_BVExtract hi lo wf vec_smt);
     expr_to_smt (Verilog.BitSelect_width vec idx _) :=
       let t_vec := Verilog.expr_type vec in
       let t_idx := Verilog.expr_type idx in
@@ -203,7 +201,7 @@ Section expr_to_smt.
       var_to_smt var
   .
 
-  Equations transfer_module_item : Verilog.module_item -> transf SMTLib.term :=
+  Equations transfer_module_item : Verilog.module_item -> transf (SMTLib.term Sort_Bool) :=
     transfer_module_item (Verilog.AlwaysComb (Verilog.BlockingAssign (Verilog.NamedExpression var) rhs)) :=
       assert_dec (In var outputs) "Assignment target must be module outputs"%string ;;
       assert_dec (List.Forall (fun n => In n inputs) (Verilog.expr_reads rhs)) "Only reads from module inputs allowed"%string ;;
@@ -213,7 +211,7 @@ Section expr_to_smt.
     transfer_module_item (Verilog.AlwaysComb _) := raise "Only single-assignment always_comb (assign) allowed"%string;
   .
 
-  Equations transfer_module_body : list Verilog.module_item -> transf (list SMTLib.term) :=
+  Equations transfer_module_body : list Verilog.module_item -> transf (list (SMTLib.term Sort_Bool)) :=
     transfer_module_body [] := ret [];
     transfer_module_body (hd :: tl) :=
       assert_dec
@@ -302,14 +300,8 @@ Definition verilog_to_smt (name_tag : TaggedVariable.Tag) (var_start : nat) (vmo
       (Verilog.module_outputs vmodule)
       (Verilog.modBody vmodule)
   in
-  let* query_wf := assert_dec _ "Query not well-formed"%string in
   inr {|
       SMT.nameMap := nameMap;
-      SMT.query :=
-        {|
-          SMTQueries.declarations := mk_declarations var_assignment;
-          SMTQueries.assertions := assertions;
-          SMTQueries.wf := query_wf;
-        |};
+      SMT.query := assertions
     |}
 .
